src/lang/Progress.v
@@ -19,16 +19,14 @@ Set Implicit Arguments.
 
 
 Lemma write_step_promise
-      lc1 mem1 loc from to val releasedc releasedm ord lc2 mem2
-      (STEP: Local.write_step lc1 mem1 loc from to val releasedc releasedm ord lc2 mem2)
+      lc1 mem1 loc from to val releasedc releasedm ord lc2 mem2 kind
+      (STEP: Local.write_step lc1 mem1 loc from to val releasedc releasedm ord lc2 mem2 kind)
       (PROMISES: lc1.(Local.promises) = Memory.bot):
   lc2.(Local.promises) = Memory.bot.
 Proof.
   inv STEP.
-  - apply Memory.ext. i. rewrite Memory.bot_get.
-    destruct (Memory.get loc0 ts (Local.promises lc2)) as [[]|] eqn:X; auto.
-    inv FULFILL. ss. inv FULFILL0. eapply Memory.remove_get_inv in X; eauto. des.
-    rewrite PROMISES, Memory.bot_get in *. congr.
+  - inv FULFILL. rewrite PROMISES in *. inv FULFILL0.
+    exploit Memory.remove_disjoint; eauto. rewrite Memory.bot_get. congr.
   - apply Memory.ext. i. rewrite Memory.bot_get.
     destruct (Memory.get loc0 ts (Local.promises lc2)) as [[]|] eqn:X; auto.
     inv FULFILL. ss. inv FULFILL0. eapply Memory.remove_get_inv in X; eauto. des.
@@ -50,47 +48,23 @@ Proof.
     inv LOCAL1. auto.
 Qed.
 
-Definition max_ts (loc:Loc.t) (mem:Memory.t): Time.t :=
-  DOMap.max_key _ (mem loc).(Cell.raw).
-
-Lemma max_ts_spec
-      loc mem
-      (CLOSED: Memory.closed mem):
-  <<GET: exists from msg, Memory.get loc (max_ts loc mem) mem = Some (from, msg)>> /\
-  <<MAX: forall ts (GET: Memory.get loc ts mem <> None), Time.le ts (max_ts loc mem)>>.
-Proof.
-  exploit (DOMap.max_key_spec _ (mem loc).(Cell.raw)); eauto.
-  { apply CLOSED. }
-  i. des. splits; eauto.
-  destruct (DOMap.find
-              (DOMap.max_key (DenseOrder.t * Message.t)
-              (Cell.raw (mem loc))) (Cell.raw (mem loc))) as [[]|] eqn:X; [|congr].
-  eexists _, _. eauto.
-Qed.
-
-(* TODO: `released` should be somehow constraint.
- * Note that we do not use `released_min`, since the update rule has `releasedr` components.
- *
- * For e.g.:
- * - released <= m.released
- * - new current <= m.released if ordering >= acqrel
- *)
 Lemma progress_promise_step
       lc1 mem1
-      loc to released val
-      (LT: Time.lt (max_ts loc mem1) to)
+      loc to val
+      (LT: Time.lt (Memory.max_ts loc mem1) to)
       (WF1: Local.wf lc1 mem1)
       (MEM1: Memory.closed mem1):
   exists promises2 mem2,
-    Local.promise_step lc1 mem1 loc (max_ts loc mem1) to val released (Local.mk lc1.(Local.commit) promises2) mem2.
+    Local.promise_step lc1 mem1 loc (Memory.max_ts loc mem1) to val (Memory.max_capability mem2) (Local.mk lc1.(Local.commit) promises2) mem2 Memory.promise_kind_add.
 Proof.
   destruct lc1. s.
-  eexists _, _. econs.
-  - s. admit.
+  exploit Memory.promise_add_exists; try apply WF1; eauto. s. i. des.
+  eexists _, _. econs; eauto.
   - refl.
   - apply WF1.
-  - apply WF1.
-Admitted.
+  - eapply Commit.future_closed; try apply WF1; eauto.
+    eapply Memory.promise_future; try apply WF1; eauto.
+Qed.
 
 Lemma progress_silent_step
       lc1 mem1
@@ -107,10 +81,10 @@ Lemma progress_read_step
       (MEM1: Memory.closed mem1)
       (PROMISES1: lc1.(Local.promises) = Memory.bot):
   exists val released lc2,
-    Local.read_step lc1 mem1 loc (max_ts loc mem1) val released ord lc2.
+    Local.read_step lc1 mem1 loc (Memory.max_ts loc mem1) val released ord lc2.
 Proof.
-  exploit (max_ts_spec loc); eauto. i. des. destruct msg.
-  exploit (@CommitFacts.read_min_spec loc (max_ts loc mem1) released); try apply WF1; i.
+  exploit (Memory.max_ts_spec loc); try apply MEM1; eauto. i. des. destruct msg.
+  exploit (@CommitFacts.read_min_spec loc (Memory.max_ts loc mem1) released); try apply WF1; i.
   { eapply MAX. inv WF1. inv COMMIT_CLOSED. inv CUR. exploit UR; eauto. i. des. rewrite x. congr. }
   { eapply MAX. inv WF1. inv COMMIT_CLOSED. inv CUR. exploit RW; eauto. i. des. rewrite x. congr. }
   { inv MEM1. exploit CLOSED; eauto. i. des. auto. }
@@ -126,47 +100,87 @@ Lemma progress_fulfill_step
       (WF1: Local.wf lc1 mem1)
       (MEM1: Memory.closed mem1)
       (GET1: Memory.get loc to mem1 = Some (from, Message.mk val releasedm))
-      (PROMISES1: lc1.(Local.promises) = Memory.singleton loc (Message.mk val releasedm) LT):
+      (PROMISES1: lc1.(Local.promises) = Memory.singleton loc (Message.mk val releasedm) LT)
+      (TO: Time.le (Capability.rw releasedc loc) to)
+      (RW: Time.lt (Capability.rw (Commit.cur (Local.commit lc1)) loc) to)
+      (REL2: Capability.le (Commit.rel (Local.commit lc1) loc) releasedc)
+      (REL: Ordering.le Ordering.acqrel ord ->
+            Capability.le (Commit.cur (Local.commit lc1)) releasedc /\
+            Time.le to (Capability.rw releasedc loc))
+      (WF: Capability.wf releasedc)
+      (CLOSED: Memory.closed_capability releasedc mem1):
   exists lc2,
     Local.fulfill_step lc1 mem1 loc from to val releasedc releasedm ord lc2.
 Proof.
-  exploit (@CommitFacts.write_min_spec loc to releasedc);
-    try apply WF1; eauto.
-  { admit. (* writable *) }
-  { admit. (* writable *) }
-  { admit. (* released <= m.released *) }
-  { admit. (* current <= m.released for acqrel *) }
-  { admit. (* closed_capability m.released *) }
-  i. des.
+  exploit (@CommitFacts.write_min_spec loc to releasedc); try apply WF1; eauto. i. des.
   eexists (Local.mk _ _). econs; eauto.
-  - rewrite PROMISES1. admit.
-  - admit.
-  - admit.
-Admitted.
+  - rewrite PROMISES1. econs.
+    apply Memory.remove_singleton.
+  - eapply CommitFacts.write_min_closed; eauto. apply WF1.
+Qed.
 
 Lemma progress_write_step
       lc1 mem1
-      loc to val releasedc releasedm ord
-      (LT: Time.lt (max_ts loc mem1) to)
+      loc to val ord
+      (LT: Time.lt (Memory.max_ts loc mem1) to)
       (WF1: Local.wf lc1 mem1)
       (MEM1: Memory.closed mem1)
       (PROMISES1: lc1.(Local.promises) = Memory.bot):
   exists lc2 mem2,
-    Local.write_step lc1 mem1 loc (max_ts loc mem1) to val releasedc releasedm ord lc2 mem2.
+    Local.write_step lc1 mem1 loc (Memory.max_ts loc mem1) to val (Memory.max_capability mem2) (Memory.max_capability mem2) ord lc2 mem2 (Some Memory.promise_kind_add).
 Proof.
   destruct lc1. ss. subst.
   exploit progress_promise_step; eauto. s. i. des.
-  assert (promises2 = Memory.singleton loc (Message.mk val releasedm) LT); subst.
-  { inv x0. ss. admit. }
-  exploit Local.promise_step_future; eauto. i. des.
-  exploit (@progress_fulfill_step (Local.mk commit (Memory.singleton loc (Message.mk val releasedm) LT))); s; eauto.
-  { inv x0. ss. inv PROMISE.
-    - eapply Memory.add_get2. eauto.
-    - eapply Memory.split_get2. eauto.
+  assert (promises2 = Memory.singleton loc (Message.mk val (Memory.max_capability mem2)) LT); subst.
+  { inv x0. ss. apply Memory.ext. i.
+    rewrite Memory.singleton_get. repeat condtac; subst.
+    - destruct (Memory.get loc to promises2) as [[]|] eqn:X.
+      + exploit Memory.promise_promises_get2; eauto. i. des; subst; eauto.
+        contradict x0. auto.
+      + exploit Memory.promise_get2; eauto. i. congr.
+    - destruct (Memory.get loc ts promises2) as [[]|] eqn:X; [|done].
+      exploit Memory.promise_promises_get2; eauto. i. des; subst; eauto.
+      + congr.
+      + rewrite Memory.bot_get in *. congr.
+    - destruct (Memory.get loc0 ts promises2) as [[]|] eqn:X; [|done].
+      exploit Memory.promise_promises_get2; eauto. i. des; subst; eauto.
+      + congr.
+      + rewrite Memory.bot_get in *. congr.
   }
-  i. des.
-  eexists _, _. econs 2; eauto.
-Admitted.
+  exploit Local.promise_step_future; eauto. i. des.
+  hexploit progress_fulfill_step; eauto; s.
+  { inv x0. ss. apply WF2. eapply Memory.promise_get2. eauto. }
+  { eauto. }
+  { inv x0. inv PROMISE. ss.
+    instantiate (1 := Memory.max_capability mem2).
+    erewrite Memory.add_max_capability; try apply MEM1; eauto.
+    s. unfold TimeMap.incr, LocFun.add. condtac; [|congr].
+    apply Time.join_spec; [|refl]. apply Time.le_lteq. auto.
+  }
+  { eapply TimeFacts.le_lt_lt; [|apply LT].
+    apply Memory.max_ts_spec. apply MEM1.
+    inv WF1. inv COMMIT_CLOSED. inv CUR. exploit RW; eauto. s. i. des. rewrite x. congr.
+  }
+  { inv x0. inv PROMISE. ss.
+    erewrite Memory.add_max_capability; try apply MEM1; eauto.
+    etrans; [|apply Capability.incr_ur_le].
+    apply Memory.max_capability_spec.
+    - inv WF1. inv COMMIT_CLOSED0. apply REL.
+    - apply MEM1.
+  }
+  { instantiate (1 := ord). i.
+    inv x0. inv PROMISE.
+    erewrite Memory.add_max_capability; try apply MEM1; eauto. ss. splits.
+    - etrans; [|apply Capability.incr_ur_le].
+      apply Memory.max_capability_spec.
+      + inv WF1. inv COMMIT_CLOSED0. apply CUR.
+      + apply MEM1.
+    - apply TimeMap.incr_ts.
+  }
+  { apply Memory.max_capability_wf. }
+  { apply Memory.max_capability_closed. apply CLOSED2. }
+  i. des. eexists _, _. econs 2; eauto.
+Qed.
 
 Lemma progress_fence_step
       lc1 mem1
